examples/opaque/server_proofs.v
@@ -72,6 +72,8 @@ wp_apply (wp_mk_nonce_freshN {[(TExp g p_s)]} (fun _ => False)%I opaque_secret
 - iIntros "%"; rewrite elem_of_singleton; iIntros "->".
   iApply minted_TExp.
     by [].
+    by [].
+    by [].
   iSplit => //.
   by iApply minted_TInt.
 - iIntros "%t".
@@ -84,7 +86,8 @@ assert (p_u ≠ p_s) as Hneq.
   apply (Hfreshp_u (TExp g p_s)).
     by rewrite elem_of_singleton.
   rewrite contra.
-  apply: subterm_TExp_exp; [done | exact: (negb_is_mul_nonce p_s) | exact: STRefl].
+  apply: subterm_TExp_exp;
+    [done | done | done | exact: (negb_is_mul_nonce p_s) | exact: STRefl].
 wp_pures.
 wp_apply wp_texp; wp_pures.
 wp_apply wp_texp.
@@ -97,6 +100,8 @@ iExists k_s, p_s, (TExp g p_s), (TExp g p_u), _.
 do !iSplit => //.
 - iApply public_TExp_iff.
     by [].
+    by [].
+    by [].
     by exact: (negb_is_mul_nonce p_s).
   do !iSplit => //.
   + by iApply minted_TInt.
@@ -105,15 +110,15 @@ do !iSplit => //.
     iNext; iModIntro; iPureIntro.
     have Nm : negb (is_mul p_s) := negb_is_mul_nonce p_s.
     rewrite (_ : TExp g p_s = TExpN g [TNonce p_s]); last by rewrite /TExpN TMulN1.
-    by rewrite exps_TExpN; [by [] | by [] | exact: invs_canceled1 Nm].
+    by rewrite exps_TExpN; [by [] | by [] | by [] | by [] | exact: invs_canceled1 Nm].
   + by iModIntro; iIntros "?"; iApply public_TInt.
 - iApply (public_sencIS _ (opN.@"AuthEnc") envelope_pred _) => //.
   1: rewrite minted_senc minted_THash minted_tag.
   1, 2: iApply minted_of_list; do !iSplit => //; iApply minted_TExp.
-  1, 3, 5: by [].
-  1-3: iSplit => //.
-  1: by rewrite minted_THash minted_tag.
-  1, 2: by iApply minted_TInt.
+  all: try by [].
+  all: try (iSplit => //).
+  all: try by rewrite minted_THash minted_tag.
+  all: try by iApply minted_TInt.
   iModIntro.
   iExists p_u, (TExp g p_u), (TExp g p_s).
   iSplit => //.
@@ -122,8 +127,10 @@ do !iSplit => //.
     iPureIntro.
     apply Hfreshp_u.
     by rewrite elem_of_singleton.
-  iApply public_TExp_exp_pred;
-    first by exact: (negb_is_mul_nonce p_s).
+  iApply public_TExp_exp_pred.
+    + by [].
+    + by [].
+    + by exact: (negb_is_mul_nonce p_s).
     + by iApply public_TInt.
     + done.
     + iApply exp_pred_intro1.
@@ -131,7 +138,7 @@ do !iSplit => //.
       iNext; iModIntro; iPureIntro.
       have Nm : negb (is_mul p_s) := negb_is_mul_nonce p_s.
       rewrite (_ : TExp g p_s = TExpN g [TNonce p_s]); last by rewrite /TExpN TMulN1.
-      by rewrite exps_TExpN; [by [] | by [] | exact: invs_canceled1 Nm].
+      by rewrite exps_TExpN; [by [] | by [] | by [] | by [] | exact: invs_canceled1 Nm].
     + done.
   iModIntro.
   rewrite public_senc_key.
@@ -164,8 +171,10 @@ do !iSplit => //.
         by rewrite /exps (expo_expN (TNonce p_s) I) factors_TMulN0.
       by move: H1; rewrite -E H2 => /Permutation_length.
     set_solver.
-  + iApply public_TExp_exp_pred;
-      first by exact: (negb_is_mul_nonce p_u).
+  iApply public_TExp_exp_pred.
+    * by [].
+    * by [].
+    * by exact: (negb_is_mul_nonce p_u).
     * by iApply public_TInt.
     * done.
     * iApply exp_pred_intro1.
@@ -173,7 +182,7 @@ do !iSplit => //.
       iNext; iModIntro; iPureIntro.
       have Nm : negb (is_mul p_u) := negb_is_mul_nonce p_u.
       rewrite (_ : TExp g p_u = TExpN g [TNonce p_u]); last by rewrite /TExpN TMulN1.
-      by rewrite exps_TExpN; [by [] | by [] | exact: invs_canceled1 Nm].
+      by rewrite exps_TExpN; [by [] | by [] | by [] | by [] | exact: invs_canceled1 Nm].
     * done.
 Qed.
 
@@ -200,6 +209,8 @@ wp_list_of_term m1; wp_pures; last first.
 rewrite !subst_list_match /=.
 wp_list_match => [uid α X_u -> | _]; last first.
   by wp_pures; iApply ("Hhl" $! None); iModIntro; do !iSplit.
+wp_eq_term X_u_one; wp_pures.
+  by iApply ("Hhl" $! None); iModIntro; do !iSplit.
 wp_bind (AList.find _ _); iApply (AList.wp_find with "Hdb"); iIntros "!> Hdb".
 case db_uid: (alist !! uid) => [file|]; wp_pures; last first.
   by iApply ("Hhl" $! None); iModIntro; do !iSplit.
@@ -217,7 +228,7 @@ wp_list_match => [k_s' p_s' P_s' P_u' envelope' e' | ]; last first.
   by [].
 symmetry in e'; inversion e'; subst; clear e'.
 rewrite public_of_list /=.
-iDestruct "Hpubm1" as "(? & ? & ? & _)".
+iDestruct "Hpubm1" as "(? & #p_α & ? & _)".
 wp_apply (wp_mk_nonce_fresh ({[X_u]} ∪ fresh) (fun _ => False)%I
                                               (fun t => opaque_secret t)%I) => //.
   iIntros "%".
@@ -239,10 +250,37 @@ set m2 := (Spec.of_list [_; _; _; _]).
 wp_apply wp_send => //.
   rewrite public_of_list => //.
   do !iSplit => //.
-  - iApply public_TExp_exp_pred => //.
-    iApply exp_pred_intro1 => //.
-    by iApply "Hexpk_s".
+  - (* [α] comes off the network, so it may well be a product.  Exponentiation
+       distributes over products, so it is enough that each factor of [α],
+       raised to [k_s], be public on its own -- and [k_s]'s seed predicate is
+       permissive enough to grant exactly that, factor by factor. *)
+    iApply public_TExp_factors.
+    iEval (rewrite public_factors) in "p_α".
+    iDestruct "p_α" as "[_ #fs]".
+    iApply big_sepL_forall; iIntros "%k %u %Hu".
+    have u_α : u ∈ factors α := list_elem_of_lookup_2 _ _ _ Hu.
+    have Nmu : negb (is_mul u) := Nmul_factors _ _ u_α.
+    iAssert (public u) as "#p_u".
+      by iApply (big_sepL_elem_of with "fs").
+    case Ei: (is_inv u); last first.
+    + have Niu : negb (is_inv u) by rewrite Ei.
+      iApply public_TExp_exp_pred => //.
+      iApply exp_pred_intro1.
+      by iApply "Hexpk_s".
+    + (* An inverse factor: [(v⁻¹) ^ k_s = (v ^ k_s)⁻¹], so peel it off. *)
+      have Nmv : negb (is_mul (TInv u)) by rewrite is_mul_TInv.
+      have Niv : negb (is_inv (TInv u)) by rewrite (is_inv_TInv _ Nmu) Ei.
+      have -> : TExp u k_s = TInv (TExp (TInv u) k_s).
+        by rewrite -TExp_TInv TInvK.
+      rewrite [public (TInv (TExp _ _))]public_TInv.
+      iAssert (public (TInv u)) as "#p_Iu".
+        by rewrite [public (TInv u)]public_TInv.
+      iApply public_TExp_exp_pred => //.
+      iApply exp_pred_intro1.
+      by iApply "Hexpk_s".
   - iApply public_TExp_iff.
+      by [].
+      by [].
       by [].
       by exact: (negb_is_mul_nonce x_s).
     do !iSplit => //.
@@ -251,7 +289,7 @@ wp_apply wp_send => //.
       iApply "Hexpx_s"; iPureIntro.
       have Nm : negb (is_mul x_s) := negb_is_mul_nonce x_s.
       rewrite (_ : TExp g x_s = TExpN g [TNonce x_s]); last by rewrite /TExpN TMulN1.
-      by rewrite exps_TExpN; [by [] | by [] | exact: invs_canceled1 Nm].
+      by rewrite exps_TExpN; [by [] | by [] | by [] | by [] | exact: invs_canceled1 Nm].
     + by rewrite public_TInt; auto.
   - iApply public_THashIS => //.
       rewrite minted_of_list /= !minted_THash !minted_tag !minted_of_list /=.
@@ -334,14 +372,12 @@ iSplit.
       rewrite elem_of_union elem_of_singleton.
       by left.
     }
-    apply subterm_TExp_exp' => //.
-    move=> contra'.
-    destruct Hfreshx_s'.
-    rewrite subterm_exp.
-    right. right.
-    exists (TInv x_s).
-    split => //.
-    apply STInv => //; by destruct x_s.
+    apply: subterm_TExp_exp_factors.
+    - exact: Hfreshx_s'.
+    - exact: (negb_is_mul_nonce x_s).
+    - by [].
+    - by move=> factors0; apply: X_u_one; rewrite -(factorsK X_u) factors0.
+    - exact: STRefl.
   + rewrite minted_of_list /=
       minted_THash minted_tag minted_of_list /=
       !minted_THash !minted_tag !minted_of_list /=
